\documentclass[11pt]{article}
\usepackage{geometry}                 
\geometry{letterpaper}                 
 \usepackage{graphicx}
\usepackage{amssymb,amsmath,amsfonts}

\newcommand{\rr}{{\mathbb R}}
 \newcommand{\F}{{\mathcal F}}
 \newcommand{\G}{{\mathcal G}}
 \newcommand{\LL}{{\mathcal L}}
 \newcommand{\M}{{\mathcal M}}
 \newcommand{\pr}{{\mathbb P}}
 \newcommand{\N}{{\mathbb N}}
\newcommand{\ex}{{\mathbb E}}
\newcommand{\ind}{{\mathbb I}}
\newcommand{\Q}{{\mathbb Q}}
\newcommand{\B}{{\mathcal B}}
\newcommand{\Fil}{{\mathcal F}}
\newcommand{\T}{{\mathcal T}}
\newcommand{\var}{{\text{Var}}}
\newcommand{\cov}{\text{Cov}}
\newcommand{\rto}{\Rightarrow}
\newcommand{\e}{{\varepsilon}}
\newcommand{\set}[1]{\left\{#1\right\}}
\newcommand{\abs}[1]{\left\vert #1\right\vert}
\newcommand{\norm}[1]{\left\| #1\right\|}
\newcommand{\charfun}{\phi_{n_k}(\frac{t}{s_n})}
\newcommand{\charind}{\frac{itX_{nk}}{s_n}}
\newcommand{\poiind}{\frac{it}{\sqrt{\lambda}}}
\newcommand{\posint}{[0,\infty]}
\parskip=10pt
  
  \begin{document}
 
\begin{center}
{\bf \large MATH 873 Homework 5}
\\
Sami Cheong
\\
\today
\end{center}
\begin{enumerate}
\item[1.] let $\{M_t,\F_t, 0 \leq t < \infty\} \in \M_2^c.$ Show that if $0 \leq s < t \leq r < u,$ then 
\[
\ex [(M_t-M_s)^2|\F_s] = \ex [M_t^2 - M_s^2|\F_s] = \ex [<M>_t - <M>_s | \F_s] \tag{1}
\]
\[
\ex [(M_t-M_s)(M_u-M_r)|\F_s] = 0 \tag{2}
\]
Proof of (1).
\begin{align*}
\ex [(M_t-M_s)^2|\F_s] & =\ex [M^2_t+M^2_s - M_sM_t -M_sM_t + M_s^2 - M_s^2|\F_s]\\ 
&=\ex [M^2_t-M_s(M_t-M_s) -M_s(M_t-M_s)- M_s^2|\F_s]\\
&=\ex [M^2_t- M_s^2|\F_s]-2\ex[M_s(M_t-M_s)|\F_s]\\
\intertext{But $M_s \in \F_s$ and $\{M_t\}$ is a martingale:}
\ex [(M_t-M_s)^2|\F_s] & = \ex [M^2_t- M_s^2|\F_s]-2\ex[M_s(M_t-M_s)|\F_s]\\
&= \ex [M^2_t- M_s^2|\F_s]-2M_s\underbrace{\ex[(M_t-M_s)|\F_s]}_{=0}\\
&=\ex[M^2_t - M_s^2|\F_s]\\
\intertext{Now, the process $\{M_t^2-<M>_t, 0\leq t < \infty\}$ is a martingale, so}
\ex[M_t^2-<M>_t -(M^2_s-<M>_s)|\F_s] & =\ex[M^t_2-M^2_s -(<M>_t-<M>_s)|\F_s] = 0,
\intertext{proving assertion (1).}
\end{align*}
Proof of (2).
\begin{align*}
\ex[(M_t-M_s)(M_u-M_r)|\F_s]& =\ex[\ex[(M_t-M_s)(M_u-M_r)|\F_r|\F_s]\\
\intertext{Since $\F_s \subset \F_r:$}
&=\ex[(M_t-M_s) \underbrace{\ex[M_u-M_r|\F_r]}_{=0}|\F_s] = 0.
\end{align*}
\end{enumerate}
\end{document}